theories/clang/lib/list.v
@@ -1,0 +1,24 @@
+(* Singly linked list *)
+
+From iris_os.clang Require Import logic tactics notations.
+
+Section proof.
+  Context `{clangG Σ}.
+
+  Fixpoint isList (l: val) (xs: list val) (t: type) :=
+    match xs with
+      | [] => True%I
+      | x::xs' => (∃ p l',
+                     ⌜ l = Vptr p ∧ typeof t x ⌝ ∗
+                     p ↦ Vpair x l' @ (Tprod t (Tptr t)) ∗ isList l' xs' t)%I
+    end.
+
+  Parameter y t: addr.
+
+  (* Definition rev_list (x: val) : stmts := *)
+  (*   y <- null ;; *)
+  (*   while (x != null) { *)
+  (*      t = !x *)
+  (*   } *)
+End proof.
+
